@prefix dcterms: <http://purl.org/dc/terms/> .
@prefix owl: <http://www.w3.org/2002/07/owl#> .
@prefix sdo: <https://schema.org/> .
@prefix skos: <http://www.w3.org/2004/02/skos/core#> .
@prefix rdfs: <http://www.w3.org/2000/01/rdf-schema#> .
@prefix tsl: <https://linked.data.gov.au/def/telephone-type/> .
@prefix vcard: <http://www.w3.org/2006/vcard/ns#> .
@prefix xsd: <http://www.w3.org/2001/XMLSchema#> .


<https://linked.data.gov.au/def/telephone-type> a owl:Ontology,
        skos:ConceptScheme ;
    dcterms:created "2020-03-25"^^xsd:date ;
    dcterms:creator <https://linked.data.gov.au/org/gsq> ;
    dcterms:modified "2020-05-13"^^xsd:date ;
    dcterms:publisher <https://linked.data.gov.au/org/gsq> ;
    dcterms:provenance "Derived from Australian Standard AS 4590.1:2017" ;
    skos:definition "The code and description that differentiates the type of telecommunications device based on the transmission service connected to the telephone network."@en ;
    skos:prefLabel "Telephone Type"@en ;
    skos:hasTopConcept 
        vcard:Cell ,
        vcard:Voice .

<https://linked.data.gov.au/org/gsq> a sdo:Organization ;
    sdo:name "Geological Survey of Queensland" ;
    sdo:url "https://www.business.qld.gov.au/industries/mining-energy-water/resources/geoscience-information/gsq"^^xsd:anyURI .

vcard:Cell a skos:Concept , vcard:TelephoneType ;
    skos:altLabel "Cell"@en,
        "Cellular"@en ;
    skos:definition "A portable telephone that can make and receive calls over a radio frequency link while the user is moving within a telephone service area."@en ;
    rdfs:isDefinedBy <https://linked.data.gov.au/def/telephone-type> ;
    skos:inScheme <https://linked.data.gov.au/def/telephone-type> ;
    skos:notation "01" ;
    skos:prefLabel "Mobile"@en ;
    skos:topConceptOf <https://linked.data.gov.au/def/telephone-type> .

vcard:Voice a skos:Concept ;
    skos:altLabel "Landline"@en , "voice"@en ;
    skos:definition "A telephone that can make and receive calls by transmission of communications signals via a cable to a fixed location."@en ;
    rdfs:isDefinedBy <https://linked.data.gov.au/def/telephone-type> ;
    skos:inScheme <https://linked.data.gov.au/def/telephone-type> ;
    skos:notation "02" ;
    skos:prefLabel "Fixed Line"@en ;
    skos:topConceptOf <https://linked.data.gov.au/def/telephone-type> .
